# Part A
The tensions in the rope connected to the boxes must have the same magnitude because of its lack of mass and lack of friction. Removing these variables also removes any possibility of the magnitudes being different.

# Part B

**INSERT FBDRB**

# Part C

First we will identify the magnitude of the forces involved. We will assume that up is positive and down is negative.

**INSERT FBDRBV**

To get the net force, we add up all the forces involved.

$\Sigma F = (m_1g - m_2g) + (-m_1g)$

$\Sigma F = (m_1g - m_2g) - (m_1g)$

$\Sigma F = (m_1g - m_2g - m_1g)$

$\Sigma F = -m_2g$ 

Now we can use Newton's Second Law to solve for acceleration.

$\Sigma F = ma$

$a = \frac{\Sigma F}{m}$

$m = m_1$

$\Sigma F = -m_2g$

$a = \frac{-m_2g}{m_1}$

$a = -\frac{m_2g}{m_1}$

# Part D

**INSERT grota**

As you can see, our graph is a horizontal line. This is because our acceleration is constant. Our acceleration is constant because we only used variables that remain constant to calculate acceleration. Mass is constant, and g is constant as well.

# Part E

$F_1 = T_1 - m_1g$

$F_1 = ma$

$T_1 - m_1g = m_1a$

# Part F

$F_2 = T_2 - m_2g$

$F_2 = ma$

$T_2 - m_2g = m_2a$

# Part G

$\tau = I\alpha$

$I = \frac{1}{2}MR^2$

$\tau = T_1R - T_2R = R(T_1 - T_2)$

$R(T_1 - T_2) = \frac{1}{2}MR^2\alpha$

$T_1 - T_2 = \frac{1}{2}MR\alpha$

$\alpha = \frac{a}{R}$

$T_1 - T_2 = \frac{1}{2}MR\frac{a}{R}$

$T_1 - T_2 = \frac{1}{2}Ma$


# Part H

$T_1 - m_1g = m_1a$ \
$T_1 = m_1a + m_1g$ \
$T_1 = m_1(a+g)$ 

$T_2 - m_2g = m_2a$ \
$T_2 = m_2a + m_2g$ \
$T_2 = m_2(a+g)$ 

$T_1 - T_2 = \frac{1}{2}Ma$ \
$m_1(a+g) - m_2(a+g) = \frac{1}{2}Ma$ \
$(a+g)(m_1-m_2) = \frac{1}{2}Ma$ \
$(m_1-m_2) = \frac{1}{2}Ma - (a+g)$ \
$(m_1-m_2) = \frac{1}{2}Ma - a - g$ \
$(m_1-m_2) = a(\frac{1}{2}M - 1) - g$ \
$(m_1-m_2) + g = a(\frac{1}{2}M - 1)$ \

$a = \frac{(m_1-m_2) + g}{(\frac{1}{2}M - 1)}$

# Part I

**INSERT grotab**

One similarity between this graph and the graph from Part D is that they both feature a straight line. This is because acceleration is constant in both cases.

One difference between this graph and the graph from Part D is that the values for acceleration are different. On Part D's graph, acceleration is equal to $-\frac{m_2g}{m_1}$, while the acceleration in Part I's graph is equal to $\frac{(m_1-m_2) + g}{(\frac{1}{2}M - 1)}$.